x86/PseudoInstructions.v
@@ -7,26 +7,67 @@ Import ListNotations.
 Local Open Scope error_monad_scope.
 Close Scope nat_scope.
 
+Context (coq_string_to_ident : string -> option ident).
+
+Definition sp_adjustment_elf64 (sg:signature) (sz:Z) :=
+  match (sg.(sig_cc)).(cc_vararg) with
+  | Some _ =>
+    let ofs := align (sz-8) 16 in
+    let sz :=  ofs + 176 (* save area *) + 8 (* return address *) in
+    let sz := align sz 16 in
+    (sz -8, ofs)
+  | None =>
+    let sz := align sz 16 in
+    (sz -8, 0)
+  end.
+
 (* Pstoreptr (linear addr ) (RAX) eval_addrmode32 *)
-Definition transf_instr (i: instruction): list instruction :=
+(** Set stack alignment to 16  *)
+Definition transf_instr (sg:signature) (i: instruction): list instruction :=
   match i with
   | Pallocframe sz ofs_ra ofs_link =>
-    let sz := align sz 8 - size_chunk Mptr in
-    let addr := linear_addr RSP (Ptrofs.unsigned ofs_link) in
-    [ Padd RAX RSP (size_chunk Mptr); Psub RSP RSP sz; Pstoreptr addr RAX]
+    (* follow Asmexpand.ml *)
+    if Archi.ptr64 then
+      let (sz, save_regs) := sp_adjustment_elf64 sg sz in
+      match (sg.(sig_cc)).(cc_vararg) with
+      | Some _ =>
+        let addr := linear_addr RSP (Ptrofs.unsigned ofs_link) in
+        let savereg_sg := mksignature [] Tvoid cc_default in
+        match coq_string_to_ident "__compcert_va_saveregs" with
+        | Some savereg_name =>          
+          [Padd RAX RSP (size_chunk Mptr);
+          Psub RSP RSP sz;
+          Pleaq R10 (linear_addr RSP save_regs);
+          Pcall_s savereg_name savereg_sg;
+          Pstoreptr addr RAX]
+        | None =>
+          [ Padd RAX RSP (size_chunk Mptr); Psub RSP RSP sz; Pstoreptr addr RAX]
+        end
+      | None =>
+        let addr := linear_addr RSP (Ptrofs.unsigned ofs_link) in
+        [ Padd RAX RSP (size_chunk Mptr); Psub RSP RSP sz; Pstoreptr addr RAX]
+      end
+    else
+      let sz := align sz 16 - size_chunk Mptr in
+      let addr := linear_addr RSP (Ptrofs.unsigned ofs_link) in
+      [ Padd RAX RSP (size_chunk Mptr); Psub RSP RSP sz; Pstoreptr addr RAX]
   | Pfreeframe fsz ofs_ra ofs_link =>
-    let sz := align fsz 8 - size_chunk Mptr in
+    if Archi.ptr64 then
+      let (sz, _) := sp_adjustment_elf64 sg fsz in
+      [Padd RSP RSP sz]
+    else
+      let sz := align fsz 16 - size_chunk Mptr in
     [ Padd RSP RSP sz ]
   | _ => [ i ]
   end.
 
-Definition transf_code (c: code) : code :=
-  concat (map transf_instr c).
+Definition transf_code (sg: signature) (c: code) : code :=
+  concat (map (transf_instr sg) c).
 
 Definition transf_function (f: function) :=
   {|
     fn_sig := fn_sig f;
-    fn_code := transf_code (fn_code f);
+    fn_code := transf_code f.(fn_sig) (fn_code f);
     fn_stacksize := fn_stacksize f;
     fn_ofs_link := fn_ofs_link f;
   |}.
